theories/TRAKHTENBROT/Sig_rem_syms.v
@@ -1,0 +1,189 @@
+(**************************************************************)
+(*   Copyright Dominique Larchey-Wendling [*]                 *)
+(*                                                            *)
+(*                             [*] Affiliation LORIA -- CNRS  *)
+(**************************************************************)
+(*      This file is distributed under the terms of the       *)
+(*         CeCILL v2 FREE SOFTWARE LICENSE AGREEMENT          *)
+(**************************************************************)
+
+Require Import List Arith Bool Lia Eqdep_dec.
+
+From Undecidability.Shared.Libs.DLW.Utils
+  Require Import utils_tac utils_list utils_nat finite.
+
+From Undecidability.Shared.Libs.DLW.Vec 
+  Require Import pos vec.
+
+From Undecidability.TRAKHTENBROT
+  Require Import notations fol_ops utils fo_terms fo_logic.
+
+Set Implicit Arguments.
+
+Local Notation ø := vec_nil.
+
+Section Sig_remove_symbols.
+
+  Variable (Σ : fo_signature).
+
+  Definition fos_nosyms : fo_signature.
+  Proof.
+    exists Empty_set (syms Σ + (unit + rels Σ))%type.
+    + intros [].
+    + intros [ s | [ [] | r ] ].
+      * exact (S (ar_syms _ s)).
+      * exact 2.
+      * exact (ar_rels _ r).
+  Defined.
+
+  Notation Σ' := fos_nosyms.
+
+  Let e : rels Σ' := inr (inl tt). 
+
+  Definition fom_nosyms X : fo_model Σ X -> fo_model Σ' X.
+  Proof.
+    intros (F,R); split.
+    + intros [].
+    + intros [s|[[]|r]].
+      * exact (fun v => vec_head v = F _ (vec_tail v)).
+      * exact (rel2_on_vec eq).
+      * exact (R r).
+  Defined. 
+
+  Notation 𝕋 := (fo_term nat (ar_syms Σ)).
+  Notation 𝔽 := (fol_form Σ).
+
+  Notation 𝕋' := (fo_term nat (ar_syms Σ')).
+  Notation 𝔽' := (fol_form Σ').
+
+  Section removing_symbols.
+
+    Let rem_syms (t : 𝕋) : 
+        { A : 𝔽' | forall X M φ ψ, 
+                          (forall n, φ n = ψ (S n))
+                       -> ψ 0 = fo_term_sem (fom_syms M) φ t 
+                      <-> fol_sem (@fom_nosyms X M) ψ A }.
+    Proof.
+      induction t as [ n | s v IHv ] using fo_term_pos_rect.
+      + exists (fol_atom Σ' e (£0##£(S n)##ø)).
+        intros X (sy,re) phi psi H2; simpl.
+        rewrite <- H2; tauto.
+      + apply vec_reif_t in IHv.
+        destruct IHv as (vB & HB).
+        set (A := fol_atom Σ' (inl s) (£(ar_syms _ s)##vec_set_pos (fun p => £ (pos2nat p)))).
+        set (f (p : pos (ar_syms _ s)) n := match n with 0 => £ (pos2nat p) | S n => £ (n+1+ar_syms _ s) end : 𝕋').
+        set (wB := vec_set_pos (fun p => (vec_pos vB p)⦃f p⦄)).
+        exists (fol_mquant fol_ex (ar_syms _ s) (A ⟑ fol_vec_fa wB)).
+        intros X M phi psi H2; simpl.
+        specialize (fun p => HB p X M).
+        destruct M as (sy,re).
+        rewrite fol_sem_mexists.
+        split.
+        * intros H3.
+          exists (vec_set_pos (fun p => fo_term_sem sy phi (vec_pos v p))); split.
+          - unfold A, fom_nosyms; simpl.
+            replace (ar_syms _ s) with (0+ar_syms _ s) at 3 by lia.
+            rewrite env_vlift_fix1; simpl; f_equal; rewrite H3; simpl; f_equal.
+            apply vec_pos_ext; intros p; rew vec; rew fot.
+            rewrite env_vlift_fix0; rew vec.
+          - rewrite fol_sem_vec_fa; intros p.
+            unfold wB; rew vec.
+            rewrite fol_sem_subst.
+            rewrite <- HB; auto.
+            2: reflexivity.
+            simpl; rew fot.
+            rewrite env_vlift_fix0; rew vec.
+            apply fo_term_sem_ext; intros n Hn.
+            replace (n+1+ar_syms _ s) with ((S n)+ar_syms _ s) by lia.
+            rewrite env_vlift_fix1; auto.
+        * intros (w & Hw1 & Hw2).
+          unfold A in Hw1; simpl in Hw1.
+          replace (ar_syms _ s) with (0+ar_syms _ s) in Hw1 at 2 by lia.
+          rewrite env_vlift_fix1 in Hw1.
+          rewrite Hw1; clear Hw1.
+          simpl; f_equal.
+          apply vec_pos_ext; intros p; rew vec.
+          rew fot.
+          unfold wB in Hw2.
+          rewrite fol_sem_vec_fa in Hw2.
+          specialize (Hw2 p); revert Hw2; rew vec; intros Hw2.
+          rewrite fol_sem_subst in Hw2.
+          rewrite <- HB with (φ := phi) in Hw2; auto.
+          intros n; simpl.
+          replace (n+1+ar_syms _ s) with ((S n)+ar_syms _ s) by lia.
+          rewrite env_vlift_fix1; auto.
+    Qed.
+
+    Definition fot_rem_syms t := proj1_sig (rem_syms t).
+
+    Fact fot_rem_syms_spec t X M φ ψ : 
+            (forall n, φ n = ψ (S n))
+         -> ψ 0 = fo_term_sem (fom_syms M) φ t 
+        <-> fol_sem (@fom_nosyms X M) ψ (fot_rem_syms t).
+    Proof. apply (proj2_sig (rem_syms t)). Qed. 
+ 
+  End removing_symbols.
+
+  Section now_formulas.
+
+    Let rem_syms (A : 𝔽) : 
+        { A' : 𝔽' | forall X M φ, 
+                          fol_sem M φ A 
+                      <-> fol_sem (@fom_nosyms X M) φ A' }.
+    Proof.
+      induction A as [ | r v | b A (A' & HA') B (B' & HB') | q A (A' & HA') ].
+      + exists ⊥; simpl; tauto.
+      + set (vB := vec_map fot_rem_syms v).
+        set (A := fol_atom Σ' (inr (inr r)) (vec_set_pos (fun p => £ (pos2nat p)))).
+        set (f (p : pos (ar_rels _ r)) n := match n with 0 => £ (pos2nat p) | S n => £ (n+ar_rels _ r) end : 𝕋').
+        set (wB := vec_set_pos (fun p => (fot_rem_syms (vec_pos v p))⦃f p⦄)).
+        exists (fol_mquant fol_ex (ar_rels _ r) (A ⟑ fol_vec_fa wB)).
+        intros X (sy,re) phi; rewrite fol_sem_mexists; split.
+        * intros H; simpl in H.
+          exists (vec_map (fo_term_sem sy phi) v); split.
+          - unfold A; simpl.
+            revert H; apply fol_equiv_ext; f_equal.
+            apply vec_pos_ext; intros p; rew vec; rew fot.
+            rewrite env_vlift_fix0; rew vec.
+          - rewrite fol_sem_vec_fa; intros p.
+            unfold wB; rew vec.
+            rewrite fol_sem_subst.
+            rewrite <- fot_rem_syms_spec; auto.
+            2: intro; reflexivity.
+            simpl.
+            rewrite env_vlift_fix0; rew vec.
+            apply fo_term_sem_ext.
+            intros; rewrite env_vlift_fix1; auto.
+        * intros (w & Hw1 & Hw2).
+          unfold A in Hw1; simpl in Hw1.
+          simpl; revert Hw1; apply fol_equiv_ext; f_equal.
+          apply vec_pos_ext; intros p; rew vec; rew fot.
+          rewrite env_vlift_fix0.
+          rewrite fol_sem_vec_fa in Hw2.
+          specialize (Hw2 p); revert Hw2; unfold wB; rew vec.
+          rewrite fol_sem_subst, <- fot_rem_syms_spec; auto.
+          2: intro; reflexivity.
+          simpl; rewrite env_vlift_fix0.
+          intros ->; apply fo_term_sem_ext.
+          intros; rewrite env_vlift_fix1; auto.
+      + exists (fol_bin b A' B').  
+        intros X M phi; simpl.
+        apply fol_bin_sem_ext; auto.
+      + exists (fol_quant q A').
+        intros X M phi.
+        simpl; apply fol_quant_sem_ext.
+        intro; auto.
+    Qed.
+
+    Definition fol_rem_syms A := proj1_sig (rem_syms A).
+
+    Fact fol_rem_syms_spec A X M φ : 
+           fol_sem M φ A 
+       <-> fol_sem (@fom_nosyms X M) φ (fol_rem_syms A).
+    Proof. apply (proj2_sig (rem_syms A)). Qed.
+
+  End now_formulas.
+
+  Check fol_rem_syms_spec.
+
+End Sig_remove_symbols.
