theories/TRAKHTENBROT/fo_definable.v
@@ -16,7 +16,7 @@ From Undecidability.Shared.Libs.DLW.Vec
   Require Import pos vec.
 
 From Undecidability.TRAKHTENBROT
-  Require Import notations fol_ops fo_terms fo_logic.
+  Require Import notations fol_ops utils fo_terms fo_logic.
 
 Set Implicit Arguments.
 
@@ -39,6 +39,12 @@ Section fo_definability.
 
   (** A FOL definable predicate is always extensional *)
 
+  Fact fot_def_ext t : fot_definable t -> forall φ ψ, (forall n, φ n = ψ n) -> t φ = t ψ.
+  Proof.
+    intros (k & _ & Hk) phi psi H.
+    rewrite <- Hk, <- Hk; apply fo_term_sem_ext; auto.
+  Qed.
+
   Fact fol_def_ext R : fol_definable R -> forall φ ψ, (forall n, φ n = ψ n) -> R φ <-> R ψ.
   Proof.
     intros (A & _ & _ & HA) phi psi H.
@@ -51,6 +57,17 @@ Section fo_definability.
   Fact fot_def_proj n : fot_definable (fun φ => φ n).
   Proof. exists (£ n); intros; split; rew fot; auto; intros _ []. Qed.
 
+  Fact fot_def_map (f : nat -> nat) t :
+           fot_definable t -> fot_definable (fun φ => t (fun n => φ (f n))).
+  Proof.
+    intros H; generalize (fot_def_ext H); revert H.
+    intros (k & H1 & H2) H3.
+    exists (fo_term_map f k); split.
+    + rewrite fo_term_syms_map; auto.
+    + intro phi; rewrite <- fo_term_subst_map; rew fot.
+      rewrite H2; apply H3; intro; rew fot; auto.
+  Qed.
+ 
   Fact fot_def_comp s v : 
         In s ls
       -> (forall p, fot_definable (fun φ => vec_pos (v φ) p))
@@ -254,7 +271,7 @@ End fo_definability.
 
 Create HintDb fol_def_db.
 
-Hint Resolve fot_def_proj fot_def_comp fol_def_True fol_def_False : fol_def_db.
+Hint Resolve fot_def_proj fot_def_map fot_def_comp fol_def_True fol_def_False : fol_def_db.
 
 Tactic Notation "fol" "def" := 
    repeat ((  apply fol_def_conj 
@@ -336,6 +353,25 @@ Section extra.
     intros [ | [ | n ] ]; simpl; fol def.
   Qed.
 
+  Fact fol_def_subst3 R t1 t2 t3 : 
+           fol_definable ls lr M (fun φ => R (φ 0) (φ 1) (φ 2))
+        -> fot_definable ls M t1
+        -> fot_definable ls M t2
+        -> fot_definable ls M t3
+        -> fol_definable ls lr M (fun φ => R (t1 φ) (t2 φ) (t3 φ)).
+  Proof.
+    intros H1 H2 H3 H4.
+    set (f n := match n with
+        | 0 => t1 
+        | 1 => t2
+        | 2 => t3
+        | _ => fun φ => φ 0
+      end).
+    change (fol_definable ls lr M (fun φ => R (f 0 φ) (f 1 φ) (f 2 φ))). 
+    apply fol_def_subst with (2 := H1) (f := f).
+    intros [ | [ | [ | n ] ] ]; simpl; fol def.
+  Qed.
+
   Let env_vec (φ : nat -> X) n := vec_set_pos (fun p => φ (@pos2nat n p)).
   Let env_env (φ : nat -> X) n k := φ (n+k).
 
@@ -354,6 +390,23 @@ Section extra.
       * unfold T; apply IHn, fol_def_fa, HR.
   Qed.
 
+  Fact fol_def_vec_ex n (R : vec X n -> (nat -> X) -> Prop) :
+           (fol_definable ls lr M (fun φ => R (env_vec φ n) (env_env φ n)))
+         -> fol_definable ls lr M (fun φ => exists v, R v φ).
+  Proof.
+    revert R; induction n as [ | n IHn ]; intros R HR.
+    + revert HR; apply fol_def_equiv; intros phi; simpl.
+      split.
+      * exists vec_nil; auto.
+      * intros (v & Hv); revert Hv; vec nil v; auto.
+    + set (T φ := exists v x, R (x##v) φ).
+      apply fol_def_equiv with (R := T).
+      * intros phi; unfold T; split.
+        - intros (v & x & Hv); exists (x##v); auto.
+        - intros (v & Hv); revert Hv; vec split v with x; exists v, x; auto.
+      * unfold T; apply IHn, fol_def_ex, HR.
+  Qed.
+
   Fact fol_def_finite_fa I (R : I -> (nat -> X) -> Prop) :
             finite_t I
          -> (forall i, fol_definable ls lr M (R i))
@@ -364,8 +417,108 @@ Section extra.
     + intros phi; apply forall_equiv; intro; split; auto.
     + apply fol_def_list_fa; auto.
   Qed.
-     
+
+  Fact fol_def_finite_ex I (R : I -> (nat -> X) -> Prop) :
+            finite_t I
+         -> (forall i, fol_definable ls lr M (R i))
+         -> fol_definable ls lr M (fun φ => exists i : I, R i φ).
+  Proof.
+    intros (l & Hl) H.
+    apply fol_def_equiv with (R := fun φ => exists i, In i l /\ R i φ).
+    + intros phi; apply exists_equiv; intro; split; auto; tauto.
+    + apply fol_def_list_ex; auto.
+  Qed.
+ 
+  Section rel_chain.
+
+    (** Definition of the following encoding ...
+        do not have to worry about managing bound
+        variable with the high lever closure operators
+
+          y ~ s1[s2[...sn[x]]] 
+      iff y ~ s1[x1] /\ x1 ~ s2[x2] /\ ... /\ xn-1 ~ sn[xn] /\ xn ~ x   
+      iff R(y,x1,s1) /\ R(x1,x2,s2) /\ ... /\ R(xn-1,xn,sn) /\ xn = x 
+     *)
+
+    Hypothesis Heq : fol_definable ls lr M (fun φ => φ 0 = φ 1).
+
+    Theorem fol_def_rel_chain I R y l x : 
+                fot_definable ls M x
+             -> fot_definable ls M y
+             -> (forall s, In s l -> fol_definable ls lr M (fun φ => R s (φ 0) (φ 1)))
+             -> fol_definable ls lr M (fun φ => @rel_chain I X R (y φ) l (x φ)).
+    Proof.
+      revert y x; induction l as [ | s l IHl ]; intros y x Hx Hy Hl; simpl.
+      + apply fol_def_subst2; auto.
+      + fol def.
+        * apply fol_def_subst2 with (R := R s); fol def.
+          apply Hl; simpl; auto.
+        * apply IHl; fol def.
+          intros; apply Hl; right; auto.
+    Qed.
+
+    Variables (R : X -> X -> X -> Prop).
+
+    Theorem fol_def_rel_chain' K y l x : 
+                fol_definable ls lr M (fun φ => R (φ 0) (φ 1) (φ 2))
+             -> fot_definable ls M x
+             -> fot_definable ls M y
+             -> forall f : K -> nat, fol_definable ls lr M (fun φ => rel_chain R (y φ) (map (fun s => φ (f s)) l) (x φ)).
+    Proof.
+      intros HR.
+      revert y x; induction l as [ | s l IHl ]; intros y x Hx Hy f; simpl.
+      + apply fol_def_subst2; auto.
+      + fol def.
+        apply fol_def_subst3; fol def.
+    Qed.
+
+  End rel_chain.
+
 End extra.
+
+Section fo_term_rsem.
+
+    Variable (sy : Type) (ar : sy -> nat)
+             (Σ : fo_signature) (ls : list (syms Σ)) (lr : list (rels Σ))
+             (X : Type) (M : fo_model Σ X).
+
+   Let env_vec (φ : nat -> X) n := vec_set_pos (fun p => φ (@pos2nat n p)).
+   Let env_env (φ : nat -> X) n k := φ (n+k).
+
+    Variable (R : forall s, vec X (ar s) -> X -> Prop).
+
+    Hypothesis H0 : fol_definable ls lr M (fun φ => φ 0 = φ 1).
+    Hypothesis HR : forall s, fol_definable ls lr M (fun φ => R (env_vec φ (ar s)) (env_env φ (ar s) 0)).
+
+    Theorem fol_def_rsem (t : fo_term nat ar) : fol_definable ls lr M (fun φ => fo_term_rsem R (fun n r => r = φ (S n)) t (φ 0)).
+    Proof.
+      induction t as [ n | s v IHv ] using fo_term_pos_rect.
+      + apply fol_def_equiv with (R := fun phi => phi 0 = phi (S n)).
+        * intros phi; rew fot; tauto.
+        * apply fol_def_subst2; auto; fol def.
+      + apply fol_def_equiv with (R := fun phi => exists w, R w (phi 0) /\ forall p, fo_term_rsem R (fun n r => r = phi (S n)) (vec_pos v p) (vec_pos w p)).
+        { symmetry; apply fo_term_rsem_fix_1. }
+        apply fol_def_vec_ex.
+        apply fol_def_conj; auto.
+        1: apply HR.
+        apply fol_def_finite_fa.
+        * apply finite_t_pos.
+        * intros p; specialize (IHv p).
+          unfold env_vec, env_env.
+          apply fol_def_equiv with (R := fun φ => fo_term_rsem R (fun n r => r = φ (ar s + S n)) (vec_pos v p) (φ (pos2nat p))).
+          - intros phi; rew vec; tauto.
+          - apply fol_def_subst with (f := fun n => 
+                match n with 
+                  | 0   => fun phi => phi (pos2nat p)
+                  | _   => fun phi => phi (ar s + n)
+                end) in IHv; auto.
+            intros []; fol def.
+    Qed.
+
+End fo_term_rsem.
+     
+
+Check fol_def_rsem.
 
 
 
