theories/TRAKHTENBROT/utils.v
@@ -1,0 +1,125 @@
+(**************************************************************)
+(*   Copyright Dominique Larchey-Wendling [*]                 *)
+(*                                                            *)
+(*                             [*] Affiliation LORIA -- CNRS  *)
+(**************************************************************)
+(*      This file is distributed under the terms of the       *)
+(*         CeCILL v2 FREE SOFTWARE LICENSE AGREEMENT          *)
+(**************************************************************)
+
+Require Import List Arith Bool Eqdep_dec.
+
+From Undecidability.Shared.Libs.DLW.Utils
+  Require Import utils_list finite.
+
+From Undecidability.TRAKHTENBROT
+  Require Import notations fol_ops.
+
+Set Implicit Arguments.
+
+Fact eq_bool_pirr (b1 b2 : bool) (H1 H2 : b1 = b2) : H1 = H2.
+Proof. apply UIP_dec, bool_dec. Qed.
+
+Fact eq_nat_pirr (n : nat) (H : n = n ) : H = eq_refl.
+Proof. apply UIP_dec, eq_nat_dec. Qed.
+
+Section graphs.
+
+  Variable (X Y : Type) (R : X -> Y -> Prop).
+
+  Definition graph_tot := forall x, ex (R x).
+  Definition graph_fun := forall x y1 y2, R x y1 -> R x y2 -> y1 = y2.
+
+  Definition is_graph_function := graph_fun /\ graph_tot.
+
+  Hypothesis (H1 : finite_t Y)
+             (H3 : forall x y, { R x y } + { ~ R x y }).
+
+  Definition graph_tot_reif : is_graph_function -> { f | forall x y, R x y <-> y = f x }.
+  Proof.
+    intros (H2 & H4). 
+    destruct finite_t_dec_choice with (3 := H4) as (f & Hf); auto.
+    exists f; intros x y; split.
+    + intros H; generalize H (Hf x); apply H2.
+    + intros ->; auto.
+  Qed.
+
+End graphs.
+
+Section rel_chain.
+
+  (* l = [s1;...;sn] 
+     rel_chain R x l y <-> y (R s1) x1 (R s2) x2 .... (R sn) xn = x 
+                       <-> y (R s1) o (R s2) o .... o (R sn) x
+  *) 
+
+  Fixpoint rel_chain I X (R : I -> X -> X -> Prop) y l x :=
+    match l with
+      | nil  => y = x
+      | s::l => exists u, R s y u /\ rel_chain R u l x
+    end.
+
+  Fact rel_chain_map I J (f : I -> J) X (R : J -> X -> X -> Prop) y l x :
+         rel_chain R y (map f l) x
+     <-> rel_chain (fun i => R (f i)) y l x.
+  Proof.
+    revert y; induction l as [ | s l IHl ]; intros y; simpl; try tauto.
+    apply exists_equiv; intro; rewrite IHl; tauto.
+  Qed.
+
+  Fact rel_chain_fold I X R f x l y :
+             (forall s, In s l -> forall u v, R s v u <-> v = f s u)
+          -> @rel_chain I X R y l x <-> y = fold_right f x l.
+  Proof.
+    revert y; induction l as [ | s l IHl ]; intros y Hl; simpl; try easy.
+    split.
+    + intros (u & H1 & H2); revert H2 H1; rewrite IHl, Hl; simpl; auto.
+      * intros -> ->; simpl; auto.
+      * intros ? ?; apply Hl; simpl; auto.
+    + intros ->.
+      exists (fold_right f x l); split.
+      * apply Hl; simpl; auto.
+      * apply IHl; auto.
+        intros ? ?; apply Hl; simpl; auto.
+  Qed.
+
+  Fact rel_chain_fun I X R l :
+             (forall s, In s l -> graph_fun (fun x y => R s y x))
+          -> graph_fun (fun x y => @rel_chain I X R y l x).
+  Proof.
+    induction l as [ | s l IHl ]; simpl; intros H x y1 y2.
+    + intros; subst; auto.
+    + intros (u1 & H1 & H2) (u2 & H3 & H4).
+      assert (forall s, In s l -> graph_fun (fun x y : X => R s y x)) as H0.
+      { intros; apply H; auto. }
+      specialize (IHl H0 _ _ _ H2 H4); subst.
+      revert H1 H3; apply H; auto.
+  Qed.
+
+  Section simul.
+
+    Variable (I X Y : Type) (R : I -> X -> X -> Prop) (T : I -> Y -> Y -> Prop)
+             (simul : X -> Y -> Prop).
+
+    Infix "⋈" := simul (at level 70, no associativity).
+
+    Fact rel_chain_simul_tot sx l x y : 
+                 (forall s x y sx, In s l -> x ⋈ y -> R s sx x -> exists sy, sx ⋈ sy /\ T s sy y)
+              -> x ⋈ y 
+              -> rel_chain R sx l x 
+              -> exists sy, sx ⋈ sy /\ rel_chain T sy l y.
+    Proof.
+      intros H Hxy; revert H sx; induction l as [ | s l IHl ]; simpl; intros H0 sx H.
+      + exists y; subst; auto.
+      + destruct H as (x' & H1 & H2).
+        destruct IHl with (2 := H2) as (y' & H3 & H4).
+        { intros ? ? ? ? ?; apply H0; auto. }
+        destruct H0 with (2 := H3) (3 := H1) as (sy & H5 & H6); auto. 
+        exists sy; split; auto.
+        exists y'; auto.
+    Qed.
+
+  End simul.
+
+End rel_chain.
+
